Dijkstra 3 -- using a 2-d allocated matrix -- is verified.

dijkstra/dijkstra_constants.v
@@ -1,6 +1,7 @@
+Require Export VST.floyd.proofauto.
 
-Definition size := 8.
-Definition inf := 1879048192.
+Definition size := 8 : Z.
+Definition inf := 1879048192 : Z.
 (* Int.max_signed - Int.max_signed/size *)
 
 Lemma size_eq: size = 8.
@@ -8,6 +9,13 @@ Proof. auto. Qed.
 
 Lemma inf_eq: inf = 1879048192. 
 Proof. auto. Qed.
+
+Lemma inf_eq2: Int.repr inf =
+               Int.sub (Int.repr 2147483647)
+                       (Int.divs (Int.repr 2147483647) (Int.repr 8)).
+Proof.
+  rewrite inf_eq. compute. trivial.
+Qed.
 
 Opaque size.
 Opaque inf.
